HybridVerifVecs/rels/cat2rel.thy
@@ -100,10 +100,12 @@ section\<open> Verification of hybrid programs \<close>
 
 subsection \<open>Verification by providing evolution\<close>
 
-definition g_evol :: "(real \<Rightarrow> 'a \<Rightarrow> 'a) \<Rightarrow> 'a pred \<Rightarrow> real set \<Rightarrow> 'a rel" ("EVOL")
+definition g_evol :: "(('a::ord) \<Rightarrow> 'b \<Rightarrow> 'b) \<Rightarrow> 'b pred \<Rightarrow> 'a set \<Rightarrow> 'b rel" ("EVOL")
   where "EVOL \<phi> G T = {(s,s') |s s'. s' \<in> g_orbit (\<lambda>t. \<phi> t s) G T}"
 
-lemma wp_g_dyn[simp]: "wp (EVOL \<phi> G T) \<lceil>Q\<rceil> = \<lceil>\<lambda>s. \<forall>t\<in>T. (\<forall>\<tau>\<in>down T t. G (\<phi> \<tau> s)) \<longrightarrow> Q (\<phi> t s)\<rceil>"
+lemma wp_g_dyn[simp]:  
+  fixes \<phi> :: "('a::preorder) \<Rightarrow> 'b \<Rightarrow> 'b"
+  shows "wp (EVOL \<phi> G T) \<lceil>Q\<rceil> = \<lceil>\<lambda>s. \<forall>t\<in>T. (\<forall>\<tau>\<in>down T t. G (\<phi> \<tau> s)) \<longrightarrow> Q (\<phi> t s)\<rceil>"
   unfolding wp_rel g_evol_def g_orbit_eq by auto
 
 
